# 语法分析之消除左递归
* 公式
```
A -> Aα | Aβ | γ
```
转化为
```
A -> γR
R -> αR | βR | ε
```
* 例子(加减法)
```
expr -> expr + term {print(+)}
     |  expr - term {print(-)}
     |  term
term -> 0 {print(0)}
     |  1 {print(1)}
       ...
     |  9 {print(9)}
```
公式对照
```
γ = term
A = expr
& = + term {print(+)}
β = - term {print(-)}

so 

expr -> term R
R -> +term {print(+)} R 
  |  -term {print(-)} R
  |  ε
term -> 0 {print(0)}
     |  1 {print(1)}
       ...
     |  9 {print(9)}
```
替换一下R
```
expr -> term rest
rest -> +term {print(+)} rest 
     |  -term {print(-)} rest 
     |  ε
term -> 0 {print(0)}
     |  1 {print(1)}
       ...
     |  9 {print(9)}
```
* 9 - 5 + 2  转 后缀
```
     expr
    /    \
  term    rest
 /  \     / |  \            \
9 {print9} - term {print-} rest
             /  \         / |  \
          5 {print5}     + term {print+}
                            /\
                           2 {print2}
```
* 伪代码实现
```
expr() {
     term();
     rest();
}
rest() {
     if (lookhead == +) {
          match(+)
          term()
          print(+)
          rest()
     } else if (lookhead == -) {
          match(-)
          term()
          print(-)
          rest()
     } else {}
}
term() {
     if (lookhead 是一个数位) {
          t = lookhead;
          match(lookhead)
          print(t)
     } else {
          语法错误
     }
}
```
